spec/pure/Varint.thy
@@ -181,6 +181,23 @@ fun varint_decode_loop :: "nat \<Rightarrow> nat \<Rightarrow> byte list \<Right
 definition varint_decode :: "byte list \<Rightarrow> (nat \<times> byte list) option" where
   "varint_decode bs = varint_decode_loop 5 0 bs"
 
+(* varint_decode_loop always returns a suffix of its input: length rest \<le> length bs. *)
+lemma varint_decode_loop_length:
+  "varint_decode_loop fuel acc bs = Some (v, rest) \<Longrightarrow> length rest \<le> length bs"
+proof (induction fuel acc bs rule: varint_decode_loop.induct)
+  case (1 acc bs) then show ?case by simp
+next
+  case (2 fuel acc) then show ?case by simp
+next
+  case (3 fuel acc b rest')
+  from 3 show ?case
+    by (auto simp: Let_def split: if_splits)
+qed
+
+lemma varint_decode_length:
+  "varint_decode bs = Some (v, rest) \<Longrightarrow> length rest \<le> length bs"
+  unfolding varint_decode_def by (rule varint_decode_loop_length)
+
 (* ---------- Base-128 digit arithmetic ---------- *)
 
 (* Interpret a big-endian digit list as a natural number. *)
